Fin2.v
@@ -1,10 +1,10 @@
 Require Export Fin.
 
 
-Fixpoint fin_lift {n} (m : Fin.t n) : Fin.t (S n) := 
+Fixpoint fin_lift1 {n} (m : Fin.t n) : Fin.t (S n) := 
     match m with
     | Fin.F1 n   => @Fin.F1 (S n)
-    | Fin.FS _ m => Fin.FS (fin_lift m)
+    | Fin.FS _ m => Fin.FS (fin_lift1 m)
     end.
 
 Fixpoint fin_to_nat {n} (m : Fin.t n):= 
@@ -13,5 +13,5 @@ Fixpoint fin_to_nat {n} (m : Fin.t n):=
     | Fin.FS _ m => S (fin_to_nat m)
     end.
 
-Coercion fin_lift   : Fin.t >-> Fin.t.
+Coercion fin_lift1  : Fin.t >-> Fin.t.
 Coercion fin_to_nat : Fin.t >-> nat.
